checkpoint

theories/ert_logic/examples/kway_merge.v
@@ -1,3 +1,4 @@
+From Coquelicot Require Import Hierarchy.
 From stdpp Require Import sorting.
 From iris.proofmode Require Export proofmode.
 From clutch.ert_logic Require Export problang_wp proofmode derived_laws ert_rules cost_models.
@@ -40,14 +41,14 @@ Definition cmp_Z_list : val :=
 Section Z_comparator_spec.
   Context `{!ert_clutchGS Σ CostTick}.
 
-  Definition is_Z_list (zs : list Z) (v : val) : iProp Σ := ⌜is_list zs v⌝.
+  Definition is_Z_list (zs : list Z) (v : val) : iProp Σ := ⌜is_list zs v⌝ ∗ ⌜Sorted Z.le zs⌝.
 
   Lemma wp_cmp_Z_list zs1 zs2 v1 v2 :
     {{{ is_Z_list zs1 v1 ∗ is_Z_list zs2 v2 }}}
       cmp_Z_list v1 v2
     {{{ RET #(bool_decide (list_Z_le zs1 zs2)); is_Z_list zs1 v1 ∗ is_Z_list zs2 v2 }}}.
   Proof.
-    iIntros (?) "[%Hzs1 %Hzs2] H".
+    iIntros (?) "[[%Hzs1 %] [%Hzs2 %]] H".
     wp_rec. wp_pures.
     wp_apply (wp_list_head _ _ zs1 with "[//]").
     iIntros (v) "[[-> ->] | (%z1 & %zs1' & -> & ->)]".
@@ -67,10 +68,30 @@ Section Z_comparator_spec.
 
 End Z_comparator_spec.
 
+(* TODO: move *)
+Section list_length_ind.
+  Variable A : Type.
+  Variable P : list A -> Prop.
+
+  Hypothesis H : ∀ xs, (∀ l, length l < length xs -> P l) -> P xs.
+
+  Theorem list_length_ind : ∀ xs, P xs.
+  Proof.
+    assert (∀ xs l : list A, length l <= length xs → P l) as H_ind.
+    { induction xs; intros l Hlen; apply H; intros l0 H0.
+      - destruct l, l0; simpl in *; lia.
+      - apply IHxs. simpl in Hlen. lia. }
+    intros xs.
+    by eapply H_ind.
+  Qed.
+End list_length_ind.
+
+Open Scope R.
+
 Program Definition Z_list_comparator : comparator (list Z) CostTick :=
   {| cmp := cmp_Z_list;
      cmp_rel := list_Z_le;
-     cmp_cost := 0%R;
+     cmp_cost := 0;
      cmp_has_key _ _ := is_Z_list;
      wp_cmp := _;
   |}.
@@ -107,51 +128,144 @@ Section kway_merge.
 
 End kway_merge.
 
+(* TODO: move *)
+Definition sum_seq (f : nat → R) (n m : nat) :=
+  foldr (Rplus ∘ f) 0 (seq n m).
+
+Lemma sum_seq_S (f : nat → R) (n m : nat) :
+  sum_seq f n (S m) = sum_seq f n m + f (n + m)%nat.
+Proof.
+  rewrite /sum_seq.
+  rewrite seq_S.
+  rewrite foldr_app /=.
+  rewrite foldr_comm_acc_strong; [lra|].
+  intros ??? =>/=. lra.
+Qed.
+
+Lemma sum_seq_nonneg f n m:
+  (∀ n, 0 <= f n) →
+  0 <= sum_seq f n m.
+Proof. Admitted.
+
+Local Hint Resolve sum_seq_nonneg : core.
+
 Section kway_merge_spec.
   Context `{!ert_clutchGS Σ CostTick} `{!min_heap Z_list_comparator}.
 
   Local Hint Resolve heap_insert_cost_nonneg : core.
   Local Hint Resolve heap_remove_cost_nonneg : core.
 
-  (** We give a rough bound by requiring, e.g., [len * (heap_insert_cost len)] credits even though,
-      in reality, only
-
-        [heap_insert_cost 0 + heap_insert_cost 1 + ... + heap_insert_cost len]
-
-      should be necessary. *)
   Definition repeat_remove_cost (zss : list (list Z)) : R :=
-    let len := length zss in
-    let total := sum_list_with length zss in
-    (** A list is removed from the heap for all elements + an extra removal for the empty lists *)
-    (total + len) * heap_remove_cost len +
-    (** A list is inserted for all elements, (except the initial head elements which are inserted as
-        part of [merge] so we should in theory subtract [len] from [total]. *)
-    total * heap_insert_cost len.
-
-  Definition merge_cost (zss : list (list Z)) : R :=
-    let len := length zss in
-    len * heap_insert_cost len + repeat_remove_cost zss.
-
+    sum_seq heap_remove_cost 0 (S (length zss)) +
+    sum_seq heap_insert_cost 0 (length zss).
 
   Lemma repeat_remove_cost_nonneg zss :
-    (0 <= repeat_remove_cost zss)%R.
+    0 <= repeat_remove_cost zss.
   Proof.
     rewrite /repeat_remove_cost.
   Admitted.
 
+  Lemma repeat_remove_cost_length zss1 zss2 :
+    length zss1 = length zss2 →
+    repeat_remove_cost zss1 = repeat_remove_cost zss2.
+  Proof. rewrite /repeat_remove_cost. by intros ->. Qed.
+
+  Local Hint Resolve Rplus_le_le_0_compat : core.
+
+  Lemma repeat_remove_cost_cons zs zss :
+    ⧖ (repeat_remove_cost (zs :: zss)) ⊢
+      ⧖ (heap_remove_cost (S (length zss))) ∗
+      ⧖ (heap_insert_cost (length zss)) ∗ ⧖ (repeat_remove_cost zss).
+  Proof.
+    rewrite {1}/repeat_remove_cost.
+    rewrite cons_length.
+    rewrite (sum_seq_S heap_remove_cost) Nat.add_0_l.
+    do 2 (rewrite etc_split; [|auto..]).
+    rewrite -!assoc.
+    rewrite (sum_seq_S heap_insert_cost) Nat.add_0_l.
+    rewrite etc_split; [|auto..].
+    iIntros "(H1 & $ & H2 & $)".
+    iCombine "H1 H2" as "H".
+    rewrite /repeat_remove_cost //.
+  Qed.
+
   Local Hint Resolve repeat_remove_cost_nonneg : core.
 
-  Lemma wp_repeat_remove h out (zss : list (list Z)) v :
-    is_list zss v →
+  Local Lemma wp_repeat_remove_aux (zss : list (list Z)) zs0 h out :
+    Forall (Sorted Z.le) zss →
+    Sorted (flip Z.le) zs0 →
+    (∀ z, z ∈ zs0 → Forall (Z.le z) (concat zss)) →
+    {{{ ⧖ (repeat_remove_cost zss) ∗ is_min_heap zss h ∗ out ↦ inject zs0 }}}
+      repeat_remove h #out
+    {{{ zs', RET #();
+        is_min_heap [] h ∗ out ↦ inject (zs0 ++ zs') ∗
+          (* TODO: the permutation is not true if [zs'] contains empty lists! *)
+        ⌜zs' ≡ₚ concat zss⌝ ∗ ⌜Sorted (flip Z.le) (zs0 ++ zs')⌝}}}.
+  Proof.
+    iIntros (Hzss Hzs0 Hle Ψ) "(Hc & Hh & Hout) HΨ".
+    iInduction (zss) as [] "IH" using list_length_ind forall (zs0 Hle Hzss Hzs0).
+    destruct zss.
+    - wp_rec; wp_pures.
+      wp_apply (wp_heap_remove with "[$Hh Hc]").
+      { rewrite /repeat_remove_cost sum_seq_S /=.
+        iApply (etc_irrel with "Hc"). cbn. lra. }
+      iIntros (?) "[(-> & % & Hh) | (% & % & % & % & % & H)]";
+        [|exfalso; by eapply Permutation_nil_cons].
+      wp_pures.
+      iApply ("HΨ" $! []). rewrite app_nil_r. by iFrame.
+    - wp_rec; wp_pures.
+      iDestruct (repeat_remove_cost_cons with "Hc") as "(Hr & Hi & Hzss)".
+      wp_apply (wp_heap_remove with "[$Hh $Hr]").
+      iIntros (w) "[(_ & % & _) | (%zs' & %u & %zss' & -> & %Hp & [%Hu %] & %Hs & Hh)]";
+        simplify_eq/=.
+      wp_pures.
+      wp_apply (wp_list_head with "[//]").
+      iIntros (w) "[[-> ->] | (% & % & -> & ->)]".
+      + wp_pures.
+        assert (length zss = length zss').
+        { by apply Permutation_length in Hp as [=]. }
+        rewrite (repeat_remove_cost_length _ zss') //.
+        wp_apply ("IH" with "[] [] [] [] Hzss Hh Hout").
+        { iPureIntro. lia. }
+        { admit. }
+        { admit. }
+        { done. }
+        iIntros (?) "(? & ?& %Heqp & %)".
+        iApply "HΨ". iFrame. iSplit; [|done].
+        iPureIntro.
+        rewrite Heqp.
+  Admitted.
+
+  Lemma wp_repeat_remove h out (zss : list (list Z)) :
     Forall (Sorted Z.le) zss →
     {{{ ⧖ (repeat_remove_cost zss) ∗ is_min_heap zss h ∗ out ↦ NONEV }}}
       repeat_remove h #out
-    {{{ zs v, RET #();
+    {{{ zs, RET #();
         is_min_heap [] h ∗ out ↦ inject zs ∗
-        ⌜is_list zs v⌝ ∗ ⌜zs ≡ₚ concat zss⌝ ∗ ⌜Sorted (flip Z.le) zs⌝}}}.
+        ⌜zs ≡ₚ concat zss⌝ ∗ ⌜Sorted (flip Z.le) zs⌝}}}.
   Proof.
-    Admitted.
+    iIntros (??) "(?&?&?) H".
+    wp_apply (wp_repeat_remove_aux _ [] with "[$]"); [done|done| |done].
+    set_solver.
+  Qed.
 
+  Definition merge_cost (zss : list (list Z)) : R :=
+    sum_seq heap_insert_cost 0 (length zss) + repeat_remove_cost zss.
+
+  Lemma etc_split_sum_seq {A} f (xs : list A) :
+    (∀ n, 0 <= f n) →
+    ⧖ (sum_seq f 0 (length xs)) ⊢ [∗ list] i ↦ _ ∈ xs, ⧖ (f i).
+  Proof.
+    iIntros (Hf).
+    iInduction xs as [|x xs] "IH" using rev_ind; [auto|].
+    rewrite app_length /=.
+    rewrite Nat.add_1_r sum_seq_S.
+    rewrite /Hierarchy.plus /=.
+    rewrite etc_split; [|auto..].
+    rewrite big_sepL_snoc.
+    iIntros "[? $]".
+    by iApply "IH".
+  Qed.
 
   Lemma wp_merge (v : val) (zss : list (list Z)) :
     is_list zss v →
@@ -162,23 +276,18 @@ Section kway_merge_spec.
   Proof.
     iIntros (Hv Hzss Ψ) "Hc HΨ".
     rewrite /merge_cost.
-    iDestruct (etc_split with "Hc") as "[Hinit Hc]".
-    { assert (0 <= length zss)%R by eauto with real. real_solver. }
-    { auto. }
+    iDestruct (etc_split with "Hc") as "[Hinit Hc]"; [auto..|].
     wp_rec.
     wp_apply wp_heap_new; [done|].
     iIntros (h) "Hh"; wp_pures.
-    rewrite etc_split_list; [|apply heap_insert_cost_nonneg].
-    wp_apply (wp_list_iter_invariant (λ _, ⧖ (heap_insert_cost (length zss))) (λ _, True)
+    rewrite etc_split_sum_seq; [|auto].
+    wp_apply (wp_list_iter_invariant (λ n _, ⧖ (heap_insert_cost n)) (λ _ _, True)
                 (λ l, is_min_heap l h) True with "[] [$Hh $Hinit //]")%I.
     { iIntros (l l' Ψ') "!# ([% ->] & _ & Hh & Hc) HΨ'".
-      rewrite app_length /=.
-      (** Here we possibly throw away some credits *)
-      iDestruct (etc_weaken _ (heap_insert_cost (length l')) with "Hc") as "Hc".
-      { split; [auto|]. apply heap_insert_cost_mono. lia. }
       wp_pures.
       wp_apply (wp_heap_insert _ l with "[$Hh $Hc]").
-      { rewrite /= /is_Z_list is_list_inject //. }
+      { rewrite /= /is_Z_list is_list_inject. iSplit; [done|].
+        by apply Forall_app in Hzss as [_ [? ?]%Forall_cons]. }
       iIntros (zss') "[Hh ->]".
       iApply "HΨ'".
       rewrite Permutation_cons_append.
@@ -187,8 +296,8 @@ Section kway_merge_spec.
     wp_pures.
     wp_alloc out as "Hout".
     wp_pures.
-    wp_apply (wp_repeat_remove with "[$Hc $Hh $Hout]"); [done|done|].
-    iIntros (zs w) "(Hh & Hout & %Hzs & %Hp & %Hsorted)".
+    wp_apply (wp_repeat_remove with "[$Hc $Hh $Hout]"); [done|].
+    iIntros (zs) "(Hh & Hout & %Hp & %Hsorted)".
     wp_pures.
     wp_load; iIntros "Hout".
     wp_apply (wp_list_rev _ _ zs with "[]").
